







Here: `- L&r - R&l - `
$$
\begin{flalign}
\delta f L&r \rightarrow  R&l \partial _x f \\
\delta g L&r \rightarrow +  asdasd R&l \partial _p g \\
\delta h L&r \rightarrow - R&l \partial _p h 
\end{flalign}
$$

Here: `- L&r - R&l - L&rR&l`
$$
\begin{flalign}
\delta f L&r \rightarrow  R&l \partial _x f  L&rR&l \\
\delta g L&r \rightarrow +  asdasd R&l \partial _p g L&rR&l \\
\delta h L&r \rightarrow - R&l \partial _p h L&rR&l \\
\end{flalign}
$$

Here: `- L&r - R&l - L&rR&lL&rR&lL&rR&lL&rR&lL&rR&lL&rR&lL&rR&lL&rR&l

$$
\begin{flalign}
\delta f L&r \rightarrow  R&l \partial _x f  L&rR&lL&rR&lL&rR&lL&rR&lL&rR&lL&rR&lL&rR&lL&rR&l \\
\delta g L&r \rightarrow +  asdasd R&l \partial _p g L&rR&lL&rR&lL&rR&l \\
\delta h L&r \rightarrow - R&l \partial _p h L&rR&lL&rR&lL&rR&l \\
\end{flalign}
$$

Here: `L&r - R&l - L&r - R&l

$$
\begin{flalign}
L&r\delta f R&l \rightarrow  L&r \partial _x f  R&l \\
L&r\delta g R&l \rightarrow +  asdasd L&r \partial _p g R&l \\
L&r\delta h R&l \rightarrow - L&r \partial _p h R&l \\
\end{flalign}
$$


Here: `L&rR&l - L&r - R&l - &

$$
\begin{flalign}
L&rR&l\delta f L&r \rightarrow  R&l \partial _x f  & \\
L&rR&l\delta g L&r \rightarrow +  asdasd R&l \partial _p g & \\
L&rR&l\delta h L&r \rightarrow - R&l \partial _p h & \\
\end{flalign}
$$


Here: `L&rR&l - L&r - R&l - &

$$
\begin{flalign}
L&r\delta f R&l \rightarrow  & \partial _x f   \\
L&r\delta g R&l \rightarrow +  asdasd & \partial _p g \\
L&r\delta h R&l \rightarrow - & \partial _p h  \\
\end{flalign}
$$

Here: `L&rR&l - L&rR&l - L&r - R&l
$$
\begin{flalign}
L&r\delta f R&lL&r \rightarrow  R&l \partial _x f   \\
L&r\delta g R&lL&r \rightarrow +  asdasd R&l \partial _p g \\
L&r\delta h R&lL&r \rightarrow - R&l \partial _p h  \\
\end{flalign}
$$

Here: ` - L&rR&l - L&r - R&l
$$
\begin{flalign}
L&r\delta f R&lL&r \rightarrow  R&l \partial _x f   \\
L&r\delta g R&lL&r \rightarrow +  asdasd R&l \partial _p g \\
L&r\delta h R&lL&r \rightarrow - R&l \partial _p h  \\
\end{flalign}
$$





